Chore: Dafny to Rust refactorings (#5513)
- extern module as attribute
- Type arguments with type bounds
- Attributes handling
- Type on Select field and TupleSelect
- Name refactoring to ensure we distinguish Dafny names from Rust names
- Binary In operator
- `NoStatementBuffer` to convert
- `GenFormals`
- `EmitNameAndActualTypeArgs` (for classes)
- `ParseAttributes`
- `GetExtractOverrideName` (to be able to model Rust options) Dafny
- `StructBuild` first argument to be an expression instead of a string
- `Apply` split into `Apply` for expressions and `ApplyType` for type
arguments
- Conversion from `Type` to `TypeParamDecl` so that we can support
bounds
- Changed `Formals` to `Fields`, and `NamelessFormals` to
`NamelessFields`
- `Visibility` has its own datatype
- Renamed `Self` to `SelfBorrowed`
- Renamed `SeltMut` to `SelfBorrowedMut`
- `Box`/`BoxNew` (for attribute annotations)
- Support for native `bool`
- `ToOwned` (used in tail recursion)
- `IsImmutableConversion`
- `Formal.self` becomes `Formal.selfBorrowed`
- `Formal.selfMut` becomes `Formal.selfBorrowedMut`
- `AssignMember` and all new variants `ExtractTuple` and `Index`
- `ExprFromType` to be able to simulate macros like expressions
- `Lambda` (makes code prettier)
- Error handling
- `Debug` trait for datatypes
- No more system object, just `std::any::Any`
- New char encoding
- `int!` macro
- Refactoring of DafatypeValue's first argument
- `constant`
- `GenIdent` refactoring

### How has this been tested?
Existing tests should just pass.

<small>By submitting this pull request, I confirm that my contribution
is made under the terms of the [MIT
license](https://github.com/dafny-lang/dafny/blob/master/LICENSE.txt).</small>

Source/DafnyCore/GeneratedFromDafny/DAST_Format.cs
@@ -11,6 +11,22 @@ using System.Collections;
 
 namespace DAST.Format {
 
+  public partial class __default {
+    public static BigInteger SeqToHeight<__T>(Dafny.ISequence<__T> s, Func<__T, BigInteger> f)
+    {
+      if ((new BigInteger((s).Count)).Sign == 0) {
+        return BigInteger.Zero;
+      } else {
+        BigInteger _763_i = Dafny.Helpers.Id<Func<__T, BigInteger>>(f)((s).Select(BigInteger.Zero));
+        BigInteger _764_j = DAST.Format.__default.SeqToHeight<__T>((s).Drop(BigInteger.One), f);
+        if ((_763_i) < (_764_j)) {
+          return _764_j;
+        } else {
+          return _763_i;
+        }
+      }
+    }
+  }
 
   public interface _IUnaryOpFormat {
     bool is_NoFormat { get; }
