Source/DafnyRuntime/DafnyRuntimeRust/src/tests/mod.rs
@@ -1,7 +1,24 @@
 // Test module
 #[cfg(test)]
 mod tests {
+    use crate::rcmut::RcMut;
+
     use crate::*;
+
+    #[test]
+    fn test_int() {
+        let x = int!(37);
+        assert_eq!(x.to_u8().unwrap(), truncate!(x.clone(), u8));
+        assert_eq!(x.to_u16().unwrap(), truncate!(x.clone(), u16));
+        assert_eq!(x.to_u32().unwrap(), truncate!(x.clone(), u32));
+        assert_eq!(x.to_u64().unwrap(), truncate!(x.clone(), u64));
+        assert_eq!(x.to_u128().unwrap(), truncate!(x.clone(), u128));
+        assert_eq!(x.to_i8().unwrap(), truncate!(x.clone(), i8));
+        assert_eq!(x.to_i16().unwrap(), truncate!(x.clone(), i16));
+        assert_eq!(x.to_i32().unwrap(), truncate!(x.clone(), i32));
+        assert_eq!(x.to_i64().unwrap(), truncate!(x.clone(), i64));
+        assert_eq!(x.to_i128().unwrap(), truncate!(x.clone(), i128));
+    }
 
     #[test]
     fn test_sequence() {
@@ -22,7 +39,7 @@ mod tests {
                 boxed,
                 length,
                 left,
-                right,
+                ..
             } => {
                 assert_eq!(*length, 6);
                 assert_eq!(unsafe { &*left.get() }.cardinality_usize(), 3);
@@ -31,15 +48,10 @@ mod tests {
             }
             _ => panic!("This should never happen"),
         }
-        let value = concat.select(0);
+        let value = concat.get_usize(0);
         assert_eq!(value, 1);
         match &concat {
-            crate::Sequence::ConcatSequence {
-                boxed,
-                length,
-                left,
-                right,
-            } => {
+            crate::Sequence::ConcatSequence { boxed, .. } => {
                 assert_eq!(
                     *boxed.as_ref().clone().borrow().as_ref().unwrap().as_ref(),
                     vec![1, 2, 3, 4, 5, 6]
@@ -57,7 +69,7 @@ mod tests {
 
     #[test]
     fn test_dafny_sequence_print() {
-        let hello = seq![
+        let hello: DafnyString = seq![
             DafnyChar('H'),
             DafnyChar('e'),
             DafnyChar('l'),
@@ -65,7 +77,7 @@ mod tests {
             DafnyChar('o')
         ];
         assert_eq!(DafnyPrintWrapper(&hello).to_string(), "Hello");
-        let hello = seq![
+        let hello: DafnyStringUTF16 = seq![
             DafnyCharUTF16(0x0048),
             DafnyCharUTF16(0x0065),
             DafnyCharUTF16(0x006c),
@@ -193,5 +205,552 @@ mod tests {
         assert_eq!(m_4b.cardinality_usize(), 4);
         assert_eq!(m_4b.contains(&3), false)
     }
+
+    #[test]
+    fn test_dafny_array() {
+        let a = array![1, 2, 3];
+        assert_eq!(crate::array::length_usize(a), 3);
+        assert_eq!(crate::array::length(a), int!(3));
+        assert_eq!(array::get_usize(a, 0), 1);
+        assert_eq!(array::get_usize(a, 1), 2);
+        assert_eq!(array::get_usize(a, 2), 3);
+        array::update_usize(a, 0, 4);
+        array::update_usize(a, 1, 5);
+        array::update_usize(a, 2, 6);
+        assert_eq!(array::get_usize(a, 0), 4);
+        assert_eq!(array::get_usize(a, 1), 5);
+        assert_eq!(array::get_usize(a, 2), 6);
+        deallocate(a);
+    }
+
+    #[test]
+    fn test_dafny_array_init() {
+        // test from_vec, and initialize
+        let mut v = Vec::new();
+        v.push(1);
+        v.push(2);
+        v.push(3);
+        let a = array::from_vec(v);
+        assert_eq!(array::length_usize(a), 3);
+        assert_eq!(array::get_usize(a, 0), 1);
+        let v2 = array::initialize_usize(3, Rc::new(|i| i + 1));
+        assert_eq!(array::length_usize(v2), 3);
+        assert_eq!(array::get_usize(v2, 0), 1);
+        assert_eq!(array::get_usize(v2, 1), 2);
+        assert_eq!(array::get_usize(v2, 2), 3);
+        array::update_usize(v2, 1, 10);
+        assert_eq!(array::get_usize(v2, 1), 10);
+
+        let v3 = array::initialize(&int!(3), Rc::new(|i| i.clone() + int!(1)));
+        assert_eq!(array::length_usize(v3), 3);
+        assert_eq!(array::get_usize(v3, 0), int!(1));
+        assert_eq!(array::get_usize(v3, 1), int!(2));
+        assert_eq!(array::get_usize(v3, 2), int!(3));
+        array::update(v3, &int!(1), int!(10));
+        assert_eq!(array::get_usize(v3, 1), int!(10));
+    }
+
+    #[test]
+    fn test_array2() {
+        let p = Array2::<DafnyInt>::placebos(&int!(3), &int!(4));
+        for i in 0..3 {
+            for j in 0..4 {
+                modify!(p).data[i][j] = MaybeUninit::new(int!(i + j));
+            }
+        }
+        let p = Array2::construct(p);
+        let p = unsafe { &*p };
+        assert_eq!(p.length0_usize(), 3);
+        assert_eq!(p.length1_usize(), 4);
+        deallocate(p);
+        // Allocate an array whose first dimension is zero
+        let p = Array2::<DafnyInt>::placebos(&int!(0), &int!(4));
+        let p = Array2::construct(p);
+        assert_eq!(read!(p).length0_usize(), 0);
+        assert_eq!(read!(p).length1_usize(), 4);
+        deallocate(p);
+    }
+
+    #[test]
+    fn test_array3() {
+        let a = Array3::<DafnyInt>::placebos(&int!(3), &int!(2), &int!(4));
+        for i in 0..3 {
+            for j in 0..2 {
+                for k in 0..4 {
+                    modify!(a).data[i][j][k] = MaybeUninit::new(DafnyInt::from(i * j + k));
+                }
+            }
+        }
+        let a = Array3::construct(a);
+        assert_eq!(read!(a).length0(), int!(3));
+        assert_eq!(read!(a).length1(), int!(2));
+        assert_eq!(read!(a).length2(), int!(4));
+        for i in 0..3 {
+            for j in 0..2 {
+                for k in 0..4 {
+                    assert_eq!(read!(a).data[i][j][k], DafnyInt::from(i * j + k));
+                }
+            }
+        }
+        deallocate(a);
+        // Even if the first two dimensions are zero, the third dimension should not be zero
+        let a = Array3::<DafnyInt>::placebos(&int!(0), &int!(0), &int!(4));
+        let a = Array3::construct(a);
+        assert_eq!(read!(a).length0(), int!(0));
+        assert_eq!(read!(a).length1(), int!(0));
+        assert_eq!(read!(a).length2(), int!(4));
+        deallocate(a);
+    }
+
+    struct ClassWrapper<T> {
+        /*var*/ t: T,
+        /*var*/ x: crate::DafnyInt,
+        /*const*/ next: *mut ClassWrapper<T>,
+        /*const*/ constant: crate::DafnyInt,
+    }
+    impl<T> AsAny for ClassWrapper<T>
+    where
+        T: 'static,
+    {
+        fn as_any(&self) -> &dyn Any {
+            self
+        }
+        fn as_any_mut(&mut self) -> &mut dyn Any {
+            self
+        }
+    }
+    impl<T: Clone> ClassWrapper<T> {
+        fn constant_plus_x(&self) -> crate::DafnyInt {
+            self.constant.clone() + self.x.clone()
+        }
+        fn increment_x(&mut self) {
+            self.x = self.x.clone() + int!(1);
+        }
+    }
+
+    impl<T: Clone + Display> ClassWrapper<T> {
+        fn constructor(t: T) -> *mut ClassWrapper<T> {
+            let this = crate::allocate::<ClassWrapper<T>>();
+            update_field_nodrop!(this, t, t);
+            update_field_nodrop!(this, next, this);
+            // If x is assigned twice, we need to keep track of whether it's assigned
+            // like in methods.
+            let mut x_assigned = false;
+            update_field_uninit!(this, x, x_assigned, int!(2));
+            update_field_uninit!(this, x, x_assigned, int!(1));
+            // If we can prove that x is assigned, we can even write this
+            modify!(this).x = int!(0);
+            update_field_nodrop!(this, constant, int!(42));
+            this
+        }
+    }
+
+    #[test]
+    #[allow(unused_unsafe)]
+    fn test_class_wrapper() {
+        let c: *mut ClassWrapper<i32> = ClassWrapper::constructor(53);
+        assert_eq!(read!(c).constant, int!(42));
+        assert_eq!(read!(c).t, 53);
+        assert_eq!(read!(c).x, int!(0));
+        assert_eq!(read!(read!(c).next).t, 53);
+        assert_eq!(read!(c).constant_plus_x(), int!(42));
+        modify!(c).increment_x();
+        assert_eq!(read!(c).constant_plus_x(), int!(43));
+        modify!(c).x = int!(40);
+        assert_eq!(read!(c).constant_plus_x(), int!(82));
+        modify!(c).t = 54;
+        assert_eq!(read!(c).t, 54);
+        let x_copy = read!(c).x.clone();
+        assert_eq!(Rc::strong_count(&x_copy.data), 2);
+        deallocate(c);
+        assert_eq!(Rc::strong_count(&x_copy.data), 1);
+    }
+
+    #[test]
+    #[allow(unused_unsafe)]
+    fn test_extern_class_wrapper_with_box() {
+        #[allow(unused_mut)]
+        let mut c = Box::new(ClassWrapper {
+            t: 53,
+            x: int!(0),
+            next: std::ptr::null_mut(),
+            constant: int!(42),
+        });
+        assert_eq!(read!(c).constant, int!(42));
+        modify!(c).increment_x();
+        assert_eq!(read!(c).constant_plus_x(), int!(43));
+        // Automatically dropped
+    }
+
+    #[test]
+    #[allow(unused_unsafe)]
+    fn test_extern_class_wrapper_with_mutable_borrow() {
+        #[allow(unused_mut)]
+        let c: &mut ClassWrapper<i32> = &mut ClassWrapper {
+            t: 53,
+            x: int!(0),
+            next: std::ptr::null_mut(),
+            constant: int!(42),
+        };
+        assert_eq!(read!(c).constant, int!(42));
+        modify!(c).increment_x();
+        assert_eq!(read!(c).constant_plus_x(), int!(43));
+        // Automatically dropped
+    }
+
+    // Requires test1 || test2
+    // We will not do that as it enables the compiler to assume that t contains a valid Rc<i32> when it does not.
+    // Prefer MaybePlacebo
+    fn assign_lazy_in_method(test1: bool, test2: bool) -> Rc<i32> {
+        let mut t = MaybePlacebo::<Rc<i32>>::new();
+        if test1 {
+            t = MaybePlacebo::from(Rc::new(5 as i32));
+        }
+        if test2 {
+            t = MaybePlacebo::from(Rc::new(
+                7 as i32 + if test1 { *MaybePlacebo::read(&t) } else { 0 },
+            ));
+        }
+        println!("{}", MaybePlacebo::read(&t));
+        MaybePlacebo::read(&t)
+    }
+
+    #[test]
+    fn assign_lazy_in_method_test() {
+        let mut t = assign_lazy_in_method(true, false);
+        assert_eq!(*t, 5);
+        t = assign_lazy_in_method(false, true);
+        assert_eq!(*t, 7);
+        t = assign_lazy_in_method(true, true);
+        assert_eq!(*t, 12);
+    }
+
+    fn override_placebo<T: Clone>(o: T, do_override: bool) {
+        let mut x: MaybePlacebo<T> = MaybePlacebo::<T>::new();
+        if do_override {
+            x = MaybePlacebo::from(o.clone());
+        }
+    }
+
+    #[test]
+    fn test_placebo() {
+        override_placebo::<Rc<BigInt>>(Rc::new(BigInt::from(1)), false);
+        override_placebo::<Rc<BigInt>>(Rc::new(BigInt::from(1)), true);
+        override_placebo::<DafnyInt>(int!(1), false);
+        override_placebo::<DafnyInt>(int!(1), true);
+        let _x: MaybePlacebo<*mut ClassWrapper<DafnyInt>> =
+            MaybePlacebo::<*mut ClassWrapper<DafnyInt>>::new();
+        //let mut f: Rc<dyn Fn(Class) -> Class> = <Rc<dyn Fn(Class) -> Class> as Placebo>::new();
+    }
+
+    #[test]
+    fn test_maybe_placebos_from() {
+        let x = (1, 2, 3, 4);
+        let (a, b, c, d) = maybe_placebos_from!(x, 0, 1, 2, 3);
+        assert_eq!(a.read(), 1);
+        assert_eq!(b.read(), 2);
+        assert_eq!(c.read(), 3);
+        assert_eq!(d.read(), 4);
+    }
+
+    #[test]
+    fn test_coercion_immutable() {
+        let o = ClassWrapper::<i32>::constructor(1);
+        let a = UpcastTo::<*mut dyn Any>::upcast_to(&o);
+        assert_eq!(cast!(a, ClassWrapper<i32>), o);
+        let seq_o = seq![o];
+        let seq_a = UpcastTo::<Sequence<*mut dyn Any>>::upcast_to(&seq_o);
+        assert_eq!(cast!(seq_a.get_usize(0), ClassWrapper<i32>), o);
+        let set_o = set! {o};
+        let set_a = UpcastTo::<Set<*mut dyn Any>>::upcast_to(&set_o);
+        assert_eq!(cast!(set_a.peek(), ClassWrapper<i32>), o);
+        let multiset_o = multiset! {o, o};
+        let multiset_a = UpcastTo::<Multiset<*mut dyn Any>>::upcast_to(&multiset_o);
+        assert_eq!(cast!(multiset_a.peek(), ClassWrapper<i32>), o);
+        let map_o = map![1 => o, 2 => o];
+        let map_a = UpcastTo::<Map<i32, *mut dyn Any>>::upcast_to(&map_o);
+        assert_eq!(cast!(map_a.get(&1), ClassWrapper<i32>), o);
+    }
+
+    #[test]
+    fn test_defaults() {
+        let set_i32 = <Set<i32> as Default>::default();
+        let seq_i32 = <Sequence<i32> as Default>::default();
+        let map_i32 = <Map<i32, i32> as Default>::default();
+        let multiset_i32 = <Multiset<i32> as Default>::default();
+        assert_eq!(set_i32.cardinality_usize(), 0);
+        assert_eq!(seq_i32.cardinality_usize(), 0);
+        assert_eq!(map_i32.cardinality_usize(), 0);
+        assert_eq!(multiset_i32.cardinality_usize(), 0);
+    }
+
+    #[test]
+    fn test_nontrivial_defaults() {
+        let set_i32 = <Set<i32> as NontrivialDefault>::nontrivial_default();
+        let seq_i32 = <Sequence<i32> as NontrivialDefault>::nontrivial_default();
+        let map_i32 = <Map<i32, i32> as NontrivialDefault>::nontrivial_default();
+        let multiset_i32 = <Multiset<i32> as NontrivialDefault>::nontrivial_default();
+        assert_eq!(set_i32.cardinality_usize(), 0);
+        assert_eq!(seq_i32.cardinality_usize(), 0);
+        assert_eq!(map_i32.cardinality_usize(), 0);
+        assert_eq!(multiset_i32.cardinality_usize(), 0);
+        let ptr_i32 = <*mut i32 as NontrivialDefault>::nontrivial_default();
+        assert_eq!(ptr_i32, std::ptr::null_mut());
+    }
+
+    #[test]
+    fn test_function_wrappers() {
+        let f: Rc<dyn Fn(i32) -> i32> = Rc::new(|i: i32| i + 1);
+        let g = f.clone();
+        let _h = seq![g];
+    }
+
+    #[test]
+    fn test_forall_exists() {
+        assert!(integer_range(int!(0), int!(10))
+            .all(Rc::new(|i: DafnyInt| i.clone() < int!(10)).as_ref()));
+        assert!(!integer_range(int!(0), int!(11))
+            .all(Rc::new(|i: DafnyInt| i.clone() < int!(10)).as_ref()));
+        assert!(!integer_range(int!(0), int!(10))
+            .any(Rc::new(|i: DafnyInt| i.clone() >= int!(10)).as_ref()));
+        assert!(integer_range(int!(0), int!(11))
+            .any(Rc::new(|i: DafnyInt| i.clone() >= int!(10)).as_ref()));
+
+        assert!(integer_range(int!(0), int!(10)).all(
+            Rc::new(|i: DafnyInt| !(i.clone() % int!(4) == int!(0))
+                || i.clone() < int!(10) && i.clone() % int!(2) == int!(0))
+            .as_ref()
+        ));
+        assert!(integer_range(int!(0), int!(11)).all(
+            Rc::new(|i: DafnyInt| !(i.clone() % int!(4) == int!(0))
+                || i.clone() < int!(10) && i.clone() % int!(2) == int!(0))
+            .as_ref()
+        ));
+        assert!(!integer_range(int!(0), int!(10)).any(
+            Rc::new(|i: DafnyInt| i.clone() % int!(4) == int!(0)
+                && i.clone() >= int!(10)
+                && i.clone() % int!(2) == int!(0))
+            .as_ref()
+        ));
+        assert!(!integer_range(int!(0), int!(11)).any(
+            Rc::new(|i: DafnyInt| i.clone() % int!(4) == int!(0)
+                && i.clone() >= int!(10)
+                && i.clone() % int!(2) == int!(0))
+            .as_ref()
+        ));
+
+        assert!(exact_range(10).all(Rc::new(|i: i32| i == 10).as_ref()));
+        assert!(exact_range(10).any(Rc::new(|i: i32| i == 10).as_ref()));
+        assert!(!exact_range(10).all(Rc::new(|i: i32| i != 10).as_ref()));
+        assert!(!exact_range(10).any(Rc::new(|i: i32| i != 10).as_ref()));
+
+        assert!(seq![1, 3, 5, 7]
+            .iter()
+            .all(Rc::new(|i: u32| i % 2 == 1).as_ref()));
+        assert!(!seq![1, 3, 5, 7]
+            .iter()
+            .any(Rc::new(|i: u32| i % 2 == 0).as_ref()));
+        assert!(!seq![1, 3, 5, 7, 8]
+            .iter()
+            .all(Rc::new(|i: u32| i % 2 == 1).as_ref()));
+        assert!(seq![1, 3, 5, 7, 8]
+            .iter()
+            .any(Rc::new(|i: u32| i % 2 == 0).as_ref()));
+
+        assert!(set! {1, 3, 5, 7}
+            .iter()
+            .cloned()
+            .all(Rc::new(|i: u32| i % 2 == 1).as_ref()));
+        assert!(!set! {1, 3, 5, 7}
+            .iter()
+            .cloned()
+            .any(Rc::new(|i: u32| i % 2 == 0).as_ref()));
+        assert!(!set! {1, 3, 5, 7, 8}
+            .iter()
+            .cloned()
+            .all(Rc::new(|i: u32| i % 2 == 1).as_ref()));
+        assert!(set! {1, 3, 5, 7, 8}
+            .iter()
+            .cloned()
+            .any(Rc::new(|i: u32| i % 2 == 0).as_ref()));
+
+        for i in set! {1, 3, 5, 7}.iter() {
+            println!("{}", i);
+        }
+
+        assert!(multiset! {1, 1, 5, 7}
+            .iter()
+            .all(Rc::new(|i: u32| i % 2 == 1).as_ref()));
+        assert!(!multiset! {1, 1, 5, 7}
+            .iter()
+            .any(Rc::new(|i: u32| i % 2 == 0).as_ref()));
+        assert!(!multiset! {1, 1, 5, 7, 8}
+            .iter()
+            .all(Rc::new(|i: u32| i % 2 == 1).as_ref()));
+        assert!(multiset! {1, 1, 5, 7, 8}
+            .iter()
+            .any(Rc::new(|i: u32| i % 2 == 0).as_ref()));
+
+        let m = map![1 => 4, 3 => 6, 5 => 8];
+        let m2 = m.clone();
+        let m3 = m.clone();
+        assert!(m
+            .clone()
+            .iter()
+            .all(Rc::new(move |i: u32| i + 3 == m2.get(&i)).as_ref()));
+        assert!(!m
+            .iter()
+            .any(Rc::new(move |i: u32| i + 2 == m3.get(&i)).as_ref()));
+        let m = map![1 => 4, 3 => 7, 5 => 7];
+        let m2 = m.clone();
+        let m3 = m.clone();
+        assert!(!m
+            .clone()
+            .iter()
+            .all(Rc::new(move |i: u32| i + 3 == m2.get(&i)).as_ref()));
+        assert!(m
+            .iter()
+            .any(Rc::new(move |i: u32| i + 2 == m3.get(&i)).as_ref()));
+    }
+
+    #[test]
+    fn test_for_loops() {
+        let mut sum: i32 = 0;
+        for i in integer_range(1, 11) {
+            sum += i;
+        }
+        assert_eq!(sum, 55);
+
+        let mut sum: i32 = 0;
+        for i in integer_range_down(11, 1) {
+            sum += i;
+        }
+        assert_eq!(sum, 55);
+
+        let mut sum: i32 = 0;
+        for i in integer_range_unbounded(1) {
+            sum += i;
+            if i == 10 {
+                break;
+            }
+        }
+        assert_eq!(sum, 55);
+
+        let mut sum: i32 = 0;
+        for i in integer_range_down_unbounded(11) {
+            sum += i;
+            if i == 1 {
+                break;
+            }
+        }
+        assert_eq!(sum, 55);
+    }
+
+    trait NodeRcMutTrait: AsAny {}
+
+    pub struct NodeRcMut {
+        val: DafnyInt,
+        next: Object<NodeRcMut>,
+    }
+    impl AsAny for NodeRcMut {
+        fn as_any(&self) -> &dyn Any {
+            self
+        }
+        fn as_any_mut(&mut self) -> &mut dyn Any {
+            self
+        }
+    }
+    impl NodeRcMut {
+        fn _ctor(this: Object<NodeRcMut>, val: DafnyInt) {
+            let mut val_assign = false;
+            let mut next_assign = false;
+            update_field_uninit_rcmut!(this.clone(), val, val_assign, val);
+            update_field_if_uninit_rcmut!(this.clone(), next, next_assign, None);
+        }
+    }
+    impl NodeRcMutTrait for NodeRcMut {}
+
+    UpcastToObject!(NodeRcMut, dyn NodeRcMutTrait);
+
+    #[test]
+    fn test_rcmut() {
+        let x: Object<NodeRcMut> = allocate_rcmut::<NodeRcMut>();
+        NodeRcMut::_ctor(x.clone(), int!(42));
+        assert_eq!(refcount!(x.clone()), 2);
+        assert_eq!(rd!(x.clone()).val, int!(42));
+        md!(x.clone()).next = x.clone();
+        assert_eq!(refcount!(x.clone()), 3);
+        assert_eq!(rd!(rd!(x.clone()).next.clone()).val, int!(42));
+        md!(rd!(x.clone()).next.clone()).next = None;
+        assert_eq!(refcount!(x.clone()), 2);
+        let y: Object<dyn Any> = x.upcast_to();
+        assert_eq!(refcount!(x.clone()), 3);
+        let z: Object<dyn NodeRcMutTrait> = x.upcast_to();
+        assert_eq!(refcount!(x.clone()), 4);
+        let a2: Object<NodeRcMut> = cast_object!(y.clone(), NodeRcMut);
+        assert_eq!(refcount!(x.clone()), 5);
+        assert_eq!(rd!(a2.clone()).val, int!(42));
+        let a3: Object<NodeRcMut> = cast_object!(z.clone(), NodeRcMut);
+        assert_eq!(refcount!(x.clone()), 6);
+        assert_eq!(rd!(a3.clone()).val, int!(42));
+        
+        let a: Object<[i32]> = rcmut::array_from_rc(Rc::new([42, 43, 44]));
+        assert_eq!(rd!(a.clone()).len(), 3);
+        assert_eq!(rd!(a.clone())[0], 42);
+        assert_eq!(rd!(a.clone())[1], 43);
+        assert_eq!(rd!(a.clone())[2], 44);
+        let b = a.clone();
+        md!(b.clone())[0] = 45;
+        assert_eq!(rd!(a.clone())[0], 45);
+    }
+
+    pub struct NodeRawMut {
+        val: DafnyInt,
+        next: *mut NodeRawMut,
+    }
+    impl NodeRawMut {
+        fn _ctor(this: *mut NodeRawMut, val: DafnyInt) {
+            let mut val_assign = false;
+            update_field_uninit!(this, val, val_assign, val);
+        }
+    }
+    impl AsAny for NodeRawMut {
+        fn as_any(&self) -> &dyn Any {
+            self
+        }
+        fn as_any_mut(&mut self) -> &mut dyn Any {
+            self
+        }
+    }
+    impl NodeRcMutTrait for NodeRawMut {}
+    
+    UpcastTo!(NodeRawMut, dyn NodeRcMutTrait);
+
+    #[test]
+    fn test_rawmut() {
+        let x: *mut NodeRawMut = allocate::<NodeRawMut>();
+        NodeRawMut::_ctor(x.clone(), int!(42));
+        //assert_eq!(refcount!(x.clone()), 2);
+        assert_eq!(read!(x.clone()).val, int!(42));
+        modify!(x.clone()).next = x.clone();
+        //assert_eq!(refcount!(x.clone()), 3);
+        assert_eq!(read!(read!(x.clone()).next.clone()).val, int!(42));
+        modify!(read!(x.clone()).next.clone()).next = std::ptr::null_mut();
+        //assert_eq!(refcount!(x.clone()), 2);
+        let y = x.upcast_to();
+        let z: *mut dyn NodeRcMutTrait = modify!(x).upcast_to();
+        let a2: *mut NodeRawMut = cast!(y, NodeRawMut);
+        let a3: *mut NodeRawMut = cast!(z, NodeRawMut);
+        //assert_eq!(refcount!(x.clone()), 3);
+        deallocate(x);
+
+        let a = array::from_native(Box::new([42, 43, 44]));
+        assert_eq!(read!(a.clone()).len(), 3);
+        assert_eq!(read!(a.clone())[0], 42);
+        assert_eq!(read!(a.clone())[1], 43);
+        assert_eq!(read!(a.clone())[2], 44);
+        let b = a.clone();
+        modify!(b.clone())[0] = 45;
+        assert_eq!(read!(a.clone())[0], 45);
+    }
 }
-// Struct containing two reference-counted fields
