Source/DafnyCore/Backends/Rust/Dafny-compiler-rust-coverage.dfy
@@ -12,39 +12,33 @@ module DafnyToRustCompilerCoverage {
     {
     }
 
+    function ConversionNum(t: Type, x: Expr): Expr {
+      Call(
+        MemberSelect(
+          MemberSelect(
+            Identifier(""),
+            "dafny_runtime"),
+          "truncate!"),
+        [x, ExprFromType(t)])
+    }
+
+    function DafnyIntLiteral(s: string): Expr {
+      Call(MemberSelect(dafny_runtime, "int!"), [LiteralInt("1")])
+    }
+
     method TestOptimizeToString() {
       var x := Identifier("x");
       var y := Identifier("y");
-      AssertCoverage(UnaryOp("&", Call(Select(x, "clone"), [], []), UnaryOpFormat.NoFormat).Optimize()
+      AssertCoverage(UnaryOp("&", Call(Select(x, "clone"), []), UnaryOpFormat.NoFormat).Optimize()
                      == UnaryOp("&", x, UnaryOpFormat.NoFormat));
-      TestNoOptimize(UnaryOp("&", Call(Select(x, "clone"), [], [y]), UnaryOpFormat.NoFormat));
+      TestNoOptimize(UnaryOp("&", Call(Select(x, "clone"), [y]), UnaryOpFormat.NoFormat));
       AssertCoverage(UnaryOp("!", BinaryOp("==", x, y, BinaryOpFormat.NoFormat),
                              CombineFormat()).Optimize() == BinaryOp("!=", x, y, BinaryOpFormat.NoFormat));
       AssertCoverage(UnaryOp("!", BinaryOp("<", x, y, BinaryOpFormat.NoFormat),
                              CombineFormat()).Optimize() == BinaryOp(">=", x, y, BinaryOpFormat.NoFormat()));
       AssertCoverage(UnaryOp("!", BinaryOp("<", x, y, ReverseFormat()),
                              CombineFormat()).Optimize() == BinaryOp("<=", y, x, BinaryOpFormat.NoFormat()));
-      AssertCoverage(
-        ConversionNum(
-          I128,
-          Call(MemberSelect(
-                 MemberSelect(MemberSelect(
-                                Identifier(""),
-                                "dafny_runtime"), "DafnyInt"), "from"), [], [LiteralInt("1")])).Optimize()
-        == LiteralInt("/*optimized*/1"));
-      AssertCoverage(
-        ConversionNum(
-          I128,
-          Call(MemberSelect(
-                 MemberSelect(MemberSelect(
-                                Identifier(""), "dafny_runtime"), "DafnyInt"), "from"), [], [LiteralString("1", false)])).Optimize()
-        == LiteralInt("/*optimized*/1"));
-      TestNoOptimize(ConversionNum(I128, Call(MemberSelect(
-                                                MemberSelect(MemberSelect(
-                                                               Identifier(""), "dafny_runtime"), "DafnyInt"), "from"), [], [x])).Optimize());
-      TestNoOptimize(ConversionNum(I128, Call(MemberSelect(
-                                                MemberSelect(MemberSelect(
-                                                               Identifier(""), "dafny_runtime"), "DafnyInt"), "from"), [], [LiteralInt("1"), LiteralInt("2")])).Optimize());
+      AssertCoverage(ConversionNum(I128, DafnyIntLiteral("1")).Optimize() == LiteralInt("1"));
       TestNoOptimize(ConversionNum(I128, x));
       AssertCoverage(StmtExpr(DeclareVar(MUT, "z", Some(I128), None), StmtExpr(AssignVar("z", y), RawExpr("return"))).Optimize()
                      == StmtExpr(DeclareVar(MUT, "z", Some(I128), Some(y)), RawExpr("return")));
@@ -53,14 +47,14 @@ module DafnyToRustCompilerCoverage {
       TestNoOptimize(x);
       TestNoOptimize(StmtExpr(x, x));
       TestNoOptimize(StmtExpr(Match(x, []), x));
-      TestNoOptimize(StmtExpr(StructBuild("x", []), x));
+      TestNoOptimize(StmtExpr(StructBuild(x, []), x));
       TestNoOptimize(StmtExpr(Tuple([]), x));
       TestNoOptimize(StmtExpr(UnaryOp("&", x, UnaryOpFormat.NoFormat), x));
       TestNoOptimize(StmtExpr(BinaryOp("&&", x, x, BinaryOpFormat.NoFormat), x));
       TestNoOptimize(StmtExpr(TypeAscription(x, I128), x));
       TestNoOptimize(StmtExpr(LiteralInt("1"), x));
-      TestNoOptimize(StmtExpr(LiteralString("1", true), x));
-      TestNoOptimize(StmtExpr(ConversionNum(I128, x), x));
+      TestNoOptimize(StmtExpr(LiteralString("2", true, false), x));
+      TestNoOptimize(StmtExpr(LiteralString("3", false, true), x));
       AssertCoverage(StmtExpr(DeclareVar(MUT, "z", Some(I128), None), StmtExpr(AssignVar("z", y), RawExpr("return"))).Optimize()
                      == StmtExpr(DeclareVar(MUT, "z", Some(I128), Some(y)), RawExpr("return")));
 
@@ -70,17 +64,15 @@ module DafnyToRustCompilerCoverage {
         Match(Identifier("x"), [MatchCase(RawPattern("abc"), Identifier("x"))]),
         StmtExpr(RawExpr("panic!()"), Identifier("a")),
         Block(RawExpr("abc")),
-        StructBuild("dummy", [AssignIdentifier("foo", Identifier("bar"))]),
-        StructBuild("dummy", [AssignIdentifier("foo", Identifier("bar")), AssignIdentifier("foo2", Identifier("bar"))]),
+        StructBuild(Identifier("dummy"), [AssignIdentifier("foo", Identifier("bar"))]),
+        StructBuild(Identifier("dummy"), [AssignIdentifier("foo", Identifier("bar")), AssignIdentifier("foo2", Identifier("bar"))]),
         Tuple([Identifier("x")]),
         UnaryOp("-", Identifier("x"), UnaryOpFormat.NoFormat),
         BinaryOp("+", Identifier("x"), Identifier("y"), BinaryOpFormat.NoFormat),
         TypeAscription(Identifier("x"), I128),
         LiteralInt("322"),
-        LiteralString("abc", true),
-        LiteralString("abc", false),
-        ConversionNum(I128, Identifier("x")),
-        ConversionNum(RawType("X"), Identifier("x")),
+        LiteralString("abc", true, false),
+        LiteralString("abc", false, true),
         DeclareVar(MUT, "abc", Some(I128), None),
         DeclareVar(CONST, "abc", None, Some(Identifier("x"))),
         AssignVar("abc", Identifier("x")),
@@ -94,8 +86,9 @@ module DafnyToRustCompilerCoverage {
         Continue(Some("l")),
         Return(None),
         Return(Some(Identifier("x"))),
-        Call(Identifier("x"), [], []),
-        Call(Identifier("x"), [I128, I32], [Identifier("x"), Identifier("y")]),
+        Call(Identifier("x"), []),
+        Call(Identifier("x"), [Identifier("x"), Identifier("y")]),
+        CallType(Identifier("x"), [I128, U32]),
         Select(Identifier("x"), "abc"),
         MemberSelect(Identifier("x"), "abc")
       ];
@@ -109,13 +102,10 @@ module DafnyToRustCompilerCoverage {
         var _ := UnaryOp("&", c, UnaryOpFormat.NoFormat()).Optimize();
         var _ := UnaryOp("!", c, UnaryOpFormat.NoFormat()).Optimize();
         var _ := ConversionNum(U8, c).Optimize();
-        var _ := ConversionNum(U8, Call(c, [], [])).Optimize();
-        var _ := ConversionNum(U8, Call(MemberSelect(c, "from"), [], [])).Optimize();
-        var _ := ConversionNum(U8, Call(MemberSelect(MemberSelect(c, "DafnyInt"), "from"), [], [])).Optimize();
-        var _ := ConversionNum(U8, Call(MemberSelect(MemberSelect(MemberSelect(c, "dafny_runtime"), "DafnyInt"), "from"), [], [])).Optimize();
-        var _ := ConversionNum(U8, Call(MemberSelect(
-                                          MemberSelect(MemberSelect(
-                                                         Identifier(""), "dafny_runtime"), "DafnyInt"), "from"), [], [c])).Optimize();
+        var _ := ConversionNum(U8, Call(c, [])).Optimize();
+        var _ := ConversionNum(U8, Call(MemberSelect(c, "int!"), [])).Optimize();
+        var _ := ConversionNum(U8, Call(MemberSelect(MemberSelect(c, "dafny_runtime"), "int!"), [])).Optimize();
+        var _ := ConversionNum(U8, Call(MemberSelect(MemberSelect(Identifier(""), "dafny_runtime"), "int!"), [c])).Optimize();
         var _ := c.RightMostIdentifier();
 
       }
@@ -128,7 +118,7 @@ module DafnyToRustCompilerCoverage {
       AssertCoverage(RawExpr("x").printingInfo.UnknownPrecedence?);
       AssertCoverage(x.printingInfo == Precedence(1));
       AssertCoverage(LiteralInt("3").printingInfo == Precedence(1));
-      AssertCoverage(LiteralString("abc", true).printingInfo == Precedence(1));
+      AssertCoverage(LiteralString("abc", true, false).printingInfo == Precedence(1));
       AssertCoverage(UnaryOp("?", x, UnaryOpFormat.NoFormat).printingInfo == SuffixPrecedence(5));
       AssertCoverage(UnaryOp("-", x, UnaryOpFormat.NoFormat).printingInfo == Precedence(6));
       AssertCoverage(UnaryOp("*", x, UnaryOpFormat.NoFormat).printingInfo == Precedence(6));
@@ -138,7 +128,7 @@ module DafnyToRustCompilerCoverage {
       AssertCoverage(UnaryOp("!!", x, UnaryOpFormat.NoFormat).printingInfo == UnknownPrecedence());
       AssertCoverage(Select(x, "name").printingInfo == PrecedenceAssociativity(2, LeftToRight));
       AssertCoverage(MemberSelect(x, "name").printingInfo == PrecedenceAssociativity(2, LeftToRight));
-      AssertCoverage(Call(x, [], []).printingInfo == PrecedenceAssociativity(2, LeftToRight));
+      AssertCoverage(Call(x, []).printingInfo == PrecedenceAssociativity(2, LeftToRight));
       AssertCoverage(TypeAscription(x, I128).printingInfo == PrecedenceAssociativity(10, LeftToRight));
       AssertCoverage(BinaryOp("*", x, y, bnf).printingInfo == PrecedenceAssociativity(20, LeftToRight));
       AssertCoverage(BinaryOp("/", x, y, bnf).printingInfo == PrecedenceAssociativity(20, LeftToRight));
